fixed the defn. of memwrite
Also, implemented the increment function.
It has a weak spec, though

examples/low-level/example1.fst
@@ -15,11 +15,12 @@ open ListSet
 val helloWorld : unit -> SST unit  (fun m -> True) (fun m0 a m1 -> True)
 let helloWorld () = (newStackFrame ())
 
+
+
 (*a good aspect of the current formulation is that the heap/stack difference
 only matters at the time of allocation. Functions like increment can be
 defined without without bothering about that distinction*)
-
-
-
-val increment : (ref int) -> SST unit  (fun m -> True) (fun m0 a m1 -> True)
-let increment r = admit ()
+val increment : r:(ref int) -> SST unit  (fun m -> (refExistsInMem r m)==true) (fun m0 a m1 -> True)
+let increment r =
+  let oldv = read r in
+  write r (oldv + 1)
